Import
```agda
{-#  OPTIONS --without-K  #-}

module thesis-4-ua where

open import thesis-4-fext public
```


Definition of univalence
Note that the type A ï¼ B , the path in the universe "type â„“",
resides in the universe "type (lsuc l)" since "type â„“ : type (lsuc l)".
```agda
tr-id : {A B : type â„“} â†’ A ï¼ B â†’ (A â†’ B)
tr-id = tr id

ï¼-â‰… : {A B : type â„“} â†’ A ï¼ B â†’ A â‰… B
ï¼-â‰… p = (â‰…pf (tr-id p)
      (Ivtbl (tr-id (p â»Â¹)) H K))
  where     -- (trâˆ™ (ğ‘–ğ‘‘ (type â„“)) (p â»Â¹) p) â»Â¹
  H : tr-id p âˆ˜ tr-id (p â»Â¹) âˆ¼ id
  H = (tr (id) p âˆ˜ tr (id) (p â»Â¹))   âˆ¼âŸ¨ happ (sym (tr-âˆ™ (id) (sym p) p) ) âŸ©
        tr (id) (p â»Â¹ âˆ™ p)           âˆ¼âŸ¨ happ (ap (\ - â†’ tr id -) (âˆ™-sym-l p)) âŸ©
        id â–¡

  K :  tr (id) (p â»Â¹) âˆ˜ tr (id) p âˆ¼ id
  K = (tr (id) (p â»Â¹) âˆ˜ tr (id) p)   âˆ¼âŸ¨ happ (sym (tr-âˆ™ (id) p (sym p)) ) âŸ©
        tr (id) (p âˆ™ p â»Â¹)    âˆ¼âŸ¨  happ (ap (\ - â†’  tr (id) -) (âˆ™-sym-r p)) âŸ©
        id â–¡

ï¼-â‰ƒ : {A B : type â„“} â†’ A ï¼ B â†’ A â‰ƒ B
ï¼-â‰ƒ = â‰…-â‰ƒ âˆ˜ ï¼-â‰…
uaâ± = ï¼-â‰ƒ

postulate
  UA : {A B : ğ“¤} â†’ equiv (ï¼-â‰ƒ {A = A} {B = B})
```


Gadgets for univalence
```agda
UA-ivtbl : {A B : ğ“¤} â†’ ivtbl (ï¼-â‰ƒ {A = A} {B = B})
UA-ivtbl = equiv-ivtbl (UA)

ua : {A B : ğ“¤} â†’ A â‰ƒ B â†’ A ï¼ B
ua = ivtbl.inv (UA-ivtbl)

ua-s : {A B : ğ“¤} â†’ (uaâ± {A = A} {B = B}) âˆ˜ (ua {A = A} {B = B}) âˆ¼ id
ua-s = ivtbl.inv-s (UA-ivtbl)

ua-r : {A B : ğ“¤} â†’ (ua {A = A} {B = B}) âˆ˜ (uaâ± {A = A} {B = B}) âˆ¼ id
ua-r = ivtbl.inv-r (UA-ivtbl)
```


Basic properties of ua

```agda
tr-ua : {X Y : ğ“¤} (E : X â‰ƒ Y)  â†’  tr-id (ua E) ï¼ (_â‰ƒ_.eqv E)
tr-ua = _â‰ƒ_.eqv  âˆ˜â‚—  (ua-s)  -- ua-s : uaâ± âˆ˜ ua âˆ¼ id  ;  eqv âˆ˜ uaâ± â‰ tr-id    âˆµ uaâ±(p) â‰  (tr-id(p), tr-id(pâ»Â¹), ...)

â‰ƒsym : {X : type â„“} {Y : type â„“'} â†’ X â‰ƒ Y â†’ Y â‰ƒ X
â‰ƒsym (â‰ƒpf eqv eqvpf) = â‰ƒpf (equiv-inv eqvpf) (equiv-inv-equiv eqvpf)

ï¼-â‰ƒ-sym : {X Y : ğ“¤} â†’ (p : X ï¼ Y) â†’ ï¼-â‰ƒ (sym p) ï¼ â‰ƒsym (ï¼-â‰ƒ p)
ï¼-â‰ƒ-sym (refl _) = refl _

ua-sym : {X Y : ğ“¤} â†’ (E : X â‰ƒ Y) â†’ ua (â‰ƒsym E) ï¼ sym (ua E)
ua-sym E
 = ua (â‰ƒsym E)        ï¼âŸ¨ ap (Î» - â†’ ua (â‰ƒsym -)) (sym (ua-s E)) âŸ©
   ua (â‰ƒsym (ï¼-â‰ƒ (ua E)))  ï¼âŸ¨ ap ua (sym (ï¼-â‰ƒ-sym (ua E))) âŸ©
   ua (ï¼-â‰ƒ (sym (ua E)))   ï¼âŸ¨ ua-r (sym (ua E)) âŸ©
   sym (ua E)  âˆ

```
